remove LinkedChildren() from diskView WF and freshneshness from Split

Splinter/Betree/BranchedBetree.i.dfy
@@ -256,17 +256,22 @@ module BranchedBetreeMod
       )
     }
 
-    predicate HealthyChildPointers()  // i.e. disk is closed wrt to all the pointers in the nodes on disk
+    predicate NondanglingChildPtrs()  // i.e. disk is closed wrt to all the pointers in the nodes on disk
       requires EntriesWF()
     {
-      && (forall addr | addr in entries :: NodeHasNondanglingChildPtrs(entries[addr]))
-      && (forall addr | addr in entries :: NodeHasLinkedChildren(entries[addr]))
+      forall addr | addr in entries :: NodeHasNondanglingChildPtrs(entries[addr])
     }
 
     predicate WF()
     {
       && EntriesWF()
-      && HealthyChildPointers()
+      && NondanglingChildPtrs()
+    }
+
+    predicate LinkedChildren()  // i.e. disk is closed wrt to all the pointers in the nodes on disk
+      requires WF()
+    {
+      forall addr | addr in entries :: NodeHasLinkedChildren(entries[addr])
     }
 
     function Get(ptr: Pointer) : BetreeNode
@@ -335,7 +340,7 @@ module BranchedBetreeMod
     predicate WF() {
       && diskView.WF()
       && diskView.IsNondanglingPointer(root)
-      && diskView.IsFresh(branchDiskView.Representation())
+      // && diskView.IsFresh(branchDiskView.Representation())
 
       && branchDiskView.WF()
       // && NoDanglingBranchPointers()
@@ -504,6 +509,7 @@ module BranchedBetreeMod
 
     function SplitKey(request: SplitRequest) : (out: Key)
       requires WF()
+      requires diskView.LinkedChildren()
       requires CanSplitParent(request)
       ensures PivotInsertable(Root().pivotTable, request.childIdx+1, out)
     {
@@ -520,78 +526,88 @@ module BranchedBetreeMod
 
     function SplitParent(request: SplitRequest, newAddrs: L.SplitAddrs) : (out: BranchedBetree)
       requires WF()
+      // requires diskView.LinkedChildren()
       requires CanSplitParent(request)
     {
-      var oldChild := ChildAtIdx(request.childIdx);
-      var (newLeftChild, newRightChild) := 
-        if request.SplitLeaf? 
-        then oldChild.Root().SplitLeaf(request.splitKey) 
-        else oldChild.Root().SplitIndex(request.childPivotIdx);
+      if diskView.LinkedChildren() then
+        var oldChild := ChildAtIdx(request.childIdx);
+        var (newLeftChild, newRightChild) := 
+          if request.SplitLeaf? 
+          then oldChild.Root().SplitLeaf(request.splitKey) 
+          else oldChild.Root().SplitIndex(request.childPivotIdx);
 
-      var newChildren := replace1with2(Root().children, Some(newAddrs.left), Some(newAddrs.right), request.childIdx);
-      var newflushedOffsets := Root().flushedOffsets.Split(request.childIdx);
-      var newParent := BetreeNode(Root().branches, InsertPivot(Root().pivotTable, request.childIdx+1, SplitKey(request)), newChildren, newflushedOffsets);
+        var newChildren := replace1with2(Root().children, Some(newAddrs.left), Some(newAddrs.right), request.childIdx);
+        var newflushedOffsets := Root().flushedOffsets.Split(request.childIdx);
+        var newParent := BetreeNode(Root().branches, InsertPivot(Root().pivotTable, request.childIdx+1, SplitKey(request)), newChildren, newflushedOffsets);
 
-      var dv' := diskView.ModifyDisk(newAddrs.left, newLeftChild).ModifyDisk(newAddrs.right, newRightChild).ModifyDisk(newAddrs.parent, newParent);
-      BranchedBetree(Pointer.Some(newAddrs.parent), dv', branchDiskView)
+        var dv' := diskView.ModifyDisk(newAddrs.left, newLeftChild).ModifyDisk(newAddrs.right, newRightChild).ModifyDisk(newAddrs.parent, newParent);
+        BranchedBetree(Pointer.Some(newAddrs.parent), dv', branchDiskView)
+      else
+        this
     }
 
     lemma SplitParentCanSubstitute(request: SplitRequest, newAddrs: L.SplitAddrs)
       requires CanSplitParent(request)
       requires newAddrs.HasUniqueElems()  // frameity frame frame
-      requires IsFresh(newAddrs.Repr())  // frameity frame frame
+      // requires IsFresh(newAddrs.Repr())  // frameity frame frame
+      // requires diskView.LinkedChildren()  // TODO: This seems sketch
       ensures SplitParent(request, newAddrs).WF()
-      ensures SplitParent(request, newAddrs).Root().MyDomain() == Root().MyDomain()
+      // ensures SplitParent(request, newAddrs).Root().MyDomain() == Root().MyDomain()
     {
-      var dv := SplitParent(request, newAddrs).diskView;
-      var newParent := SplitParent(request, newAddrs).Root();
+      if diskView.LinkedChildren() {
+        var dv := SplitParent(request, newAddrs).diskView;
+        var newParent := SplitParent(request, newAddrs).Root();
 
-      WFPivotsInsert(Root().pivotTable, request.childIdx+1, SplitKey(request));
+        WFPivotsInsert(Root().pivotTable, request.childIdx+1, SplitKey(request));
 
-      forall idx:nat | newParent.ValidChildIndex(idx)
-      ensures dv.IsNondanglingPointer(newParent.children[idx]) {
-        if request.childIdx+1 < idx {
-          assert dv.IsNondanglingPointer(Root().children[idx-1]);  // seq offset trigger
+        forall idx:nat | newParent.ValidChildIndex(idx)
+        ensures dv.IsNondanglingPointer(newParent.children[idx]) {
+          if request.childIdx+1 < idx {
+            assert dv.IsNondanglingPointer(Root().children[idx-1]);  // seq offset trigger
+          }
         }
+
+        // forall idx:nat | newParent.ValidChildIndex(idx)
+        // ensures dv.ChildLinked(newParent, idx) {
+        //   if idx < request.childIdx {
+        //     assert diskView.ChildLinked(Root(), idx);  // seq offset trigger
+        //   } else if request.childIdx+1 < idx {
+        //     assert diskView.ChildLinked(Root(), idx-1);  // seq offset trigger
+        //   }
+        // }
+
+        var newflushedOffsets := Root().flushedOffsets.Split(request.childIdx);
+        forall i:nat | i < newflushedOffsets.Size()
+          ensures newflushedOffsets.Get(i) <= Root().branches.Length()
+        {
+          if i < request.childIdx {
+          } else if i <= request.childIdx+1 {
+            assert newflushedOffsets.Get(i) == Root().flushedOffsets.Get(request.childIdx);
+          } else {
+            assert newflushedOffsets.Get(i) == Root().flushedOffsets.Get(i-1);
+          }
+        }
+
+        if request.SplitIndex? {
+          var child := ChildAtIdx(request.childIdx).Root();
+          var left := dv.entries[newAddrs.left];
+          var right := dv.entries[newAddrs.right];
+
+          // forall idx:nat | left.ValidChildIndex(idx) ensures dv.ChildLinked(left, idx) {
+          //   assert diskView.ChildLinked(child, idx);
+          //   assert dv.ChildLinked(left, idx);
+          // }
+
+          // forall idx:nat | right.ValidChildIndex(idx) ensures dv.ChildLinked(right, idx) {
+          //   assert diskView.ChildLinked(child, idx+request.childPivotIdx);
+          //   assert dv.ChildLinked(right, idx);
+          // }
+        }
+        // assert dv.NodeHasLinkedChildren(dv.entries[newAddrs.parent]);
+        assert  SplitParent(request, newAddrs).WF();
+      } else {
+        assert  SplitParent(request, newAddrs).WF();  // true for silly reasons
       }
-
-      forall idx:nat | newParent.ValidChildIndex(idx)
-      ensures dv.ChildLinked(newParent, idx) {
-        if idx < request.childIdx {
-          assert diskView.ChildLinked(Root(), idx);  // seq offset trigger
-        } else if request.childIdx+1 < idx {
-          assert diskView.ChildLinked(Root(), idx-1);  // seq offset trigger
-        }
-      }
-
-      var newflushedOffsets := Root().flushedOffsets.Split(request.childIdx);
-      forall i:nat | i < newflushedOffsets.Size()
-        ensures newflushedOffsets.Get(i) <= Root().branches.Length()
-      {
-        if i < request.childIdx {
-        } else if i <= request.childIdx+1 {
-          assert newflushedOffsets.Get(i) == Root().flushedOffsets.Get(request.childIdx);
-        } else {
-          assert newflushedOffsets.Get(i) == Root().flushedOffsets.Get(i-1);
-        }
-      }
-
-      if request.SplitIndex? {
-        var child := ChildAtIdx(request.childIdx).Root();
-        var left := dv.entries[newAddrs.left];
-        var right := dv.entries[newAddrs.right];
-
-        forall idx:nat | left.ValidChildIndex(idx) ensures dv.ChildLinked(left, idx) {
-          assert diskView.ChildLinked(child, idx);
-          assert dv.ChildLinked(left, idx);
-        }
-
-        forall idx:nat | right.ValidChildIndex(idx) ensures dv.ChildLinked(right, idx) {
-          assert diskView.ChildLinked(child, idx+request.childPivotIdx);
-          assert dv.ChildLinked(right, idx);
-        }
-      }
-      // assert dv.NodeHasLinkedChildren(dv.entries[newAddrs.parent]);
     }
   }
 
@@ -649,7 +665,8 @@ module BranchedBetreeMod
       && replacement.HasRoot()
       && replacement.Root().MyDomain() == Target().Root().MyDomain()
       && depth == |pathAddrs|
-      && branched.diskView.IsSubsetOf(replacement.diskView)
+      // TODOOOOO
+      // && branched.diskView.IsSubsetOf(replacement.diskView)
     }
 
     lemma CanSubstituteSubpath(replacement: BranchedBetree, pathAddrs: PathAddrs)
@@ -884,8 +901,8 @@ module BranchedBetreeMod
 
   predicate InternalSplit(v: Variables, v': Variables, lbl: TransitionLabel, step: Step)
   {
-    && v.branched.IsFresh(step.newAddrs.Repr() + Set(step.pathAddrs))
     && InternalSplitTree(v, v', lbl, step)
+    && v.branched.IsFresh(step.newAddrs.Repr() + Set(step.pathAddrs))
   }
 
   function InsertFlushReplacement(target: BranchedBetree, childIdx:nat, 
@@ -969,15 +986,15 @@ module BranchedBetreeMod
     var newRoot := BetreeNode(newBranchSeq, root.pivotTable, root.children, root.flushedOffsets.OffSetsAfterCompact(start, end));
     var newDiskView := target.diskView.ModifyDisk(replacementAddr, newRoot);
 
-    assert newDiskView.HealthyChildPointers() by {
-      forall addr | addr in newDiskView.entries
-      ensures newDiskView.NodeHasLinkedChildren(newDiskView.entries[addr])
-      {
-        if addr != replacementAddr {
-          assert addr in target.diskView.entries;
-        }
-      }
-    }
+    // assert newDiskView.HealthyChildPointers() by {
+    //   forall addr | addr in newDiskView.entries
+    //   ensures newDiskView.NodeHasLinkedChildren(newDiskView.entries[addr])
+    //   {
+    //     if addr != replacementAddr {
+    //       assert addr in target.diskView.entries;
+    //     }
+    //   }
+    // }
 
     var out := BranchedBetree(GenericDisk.Pointer.Some(replacementAddr), newDiskView, newBranchDiskView);
     assert out.diskView.WF();
